$f_1: x =  (-\infty, \infty)$
$f_2: x = \mathbb{R} - \{1.5\}$
$f_3: x = (-\infty, \infty)$
$f_4: x = \langle 2, \infty)$
$f_5 : x =\langle 2, \infty) - \{0\}$
$f_6 : x = \langle -3, \infty) - \{-7\}$
$f_7 : x = (-3, \infty) - \{-7\}$

---

$d=7$
$f_1: y = 3x-4$
$f_1^{-1} : x = \frac{y+4}{3}$
ano

//

$d = 5$
$f_2: y = -5$
$f_2^{-1}: x = -5$
ne

//

$d = 0$
$f_3:y = \frac{1}{x+3}$
$f_3^{-1}: x = \frac{1}{y}-3$
ne

//

$d=-4$
$f_4:y=\frac{x+1}{x-2}$
$f_4^{-1} : x = -y+1$
ano

//
$d = \frac{1}{2}$
$f_5 : y = \frac{1}{x^2-1}$
$f_5^{-1} : x = \sqrt{\frac{1}{y}-1}$

ano


---

b = 4

//
b = 12
//
a = -3
//
a = 4

---

0;3 , -3;0
3 = 0a+ b
0 = -3a + b


---
-1 , 3
4, -2

3 = -1a + b
-2 = 4a + b
a = -1
3 = 1 + b
-2 = -4 + b

y = -x + 2

---
 2 = 3a  + b
 -1 = 4a + b 
a -3
2 = -9 + b
-1 = -12 + b
b = 11 

y = ax + b
y = -3x + 11


---

y = ax+b

-1 = a + b
5 = -2a + b
b = 5+2a
-1 = a + 5 + 2a
-1 = 3a + 5
3a = -6
a = -2

5 = -2 x -2 + b
5 = 4 + b
b =  1

y = -2x + 1


---

[0,3]  [ 1,0]

3 = a0 + b
0 = 1a + b
b = 3
a = -3

y = -3x + 3

---

[0,-2]  [ 1,1]

y = ax + b
-2 = 0 + b
b = -2 

1 = 1a - 2
a = 3

y = 3x -2

---

y = -1x + 4

y = 0
x - 4


y = 4
x = 0

---

$y=\frac{x}{2}+3$
y = 2

$2-3 = \frac{x}{2}$
$-1 = \frac{-2}{2}$
x -2


y = 0
0 = 2x -3
x = 1,5

y = 2
2 = 2x - 3
x = 2, 5

---

y = 0
0 = -6/3 + 2

y = 0/3 + 2
y = 2

y = 0

0 = 2(1-x)-2
x = 0


x = 2

y = 2(-1)-2
y = -2-2
y = -4

---


x = 0
y = 3 - (0 + 1)/2
y = 2,5


---



y = ax + b

-2 = 2a + b
-1 = 4a + b
a = 1/2
b = -3

---

$\frac{x+2}{x-1} = \frac{x+6}{x+2}$
$(x+2) * (x+2) = (x+6) * (x-1)$
$x^2 + 4x + 4 = x^2 +5x - 6$
$4x +4 = 5x -6$
$-x = -6 + 4$
$-x = -2$
$x = 2$

---


$\frac{2x+1}{x-3}=\frac{4x+2}{2x-1}$
$(2x+1)(2x-1)=(4x+2)(x-3)$
$4x^2-1 = 4x^2 + 2x - 12x - 6$ 
$-1 = -10x - 6$
$10x = -5$
$x = -\frac{1}{2}$

---


$\frac{x+3}{x-2}=4+\frac{5}{x-2}$
$(x+3)= 4(x-2)+5$
$6 = 3x$
$x = 2$

---

$\frac{x+4}{x+5}=2-\frac{1}{x+5}$
$x+4=2(x+5)-1$
$x+4 = 2x + 9$
$3x = 13$


