
$|x-1| + |x+1|  = 3$





$K_1$
$-(x-1)-(x+1)=3$
$-x+1-x-1=3$
$-2x = 3$
$-2x = 3$
$2x = -3$
$x = -\frac{3}{2}$
$K_1 = \{-\frac{3}{2}\}$


$K_2$
$(x-1)-(x+1)=3$
$x-1-x-1=3$
$-2 = 3$
$K_2=\{\varnothing\}$



$K_3$
$-(x-1)+(x+1)=3$
$-x+1+x+1=3$
$2 = 3$
$K_3=\{\varnothing\}$

$K_4$
$(x-1)+(x+1)=3$
$x-1+x+1 = 3$
$2x = 3$
$x = \frac{3}{2}$


---

$3*|x-5|+2*(x+1) = 2$



$K_1$
$3*(x-5)+2*(x+1)=2$
$3x-15+2x+2 = 2$
$5x - 13 = 2$
$5x = 15$
$x = 3$


$K_2$
$3*-(x-5)+2*(x+1)=2$
$-3x+15+2x+2=2$
$-1x + 17 = 2$
$x = 15$


---

