


a.

$x+2y=5$
$2x+y = 7$
$x + 2y = 5$
$2x - 7 = -y$
$x+2(-2x+7) = 5$
$x -4x+14=5$
$-3x = -9$
$3x = 9$
$x = 3$
$2*3 + y = 7$
$6 + y = 7$
$y = 1$

zk
$3+2*1 = 5$

---

b

1.
$3x+2y = 25$
$3x+2(2x-12) = 25$
$3x +4x - 24 = 25$
$7x = 49$
$x = 7$



2. 

$2x-y = 12$
$2x-12 = y$
$98 - y = 12$
$-y = 12 - 98$
$-y = -76$
$y = 76$


zk. 

$98 - 76= 12$

---


c/

1.
$2x-3y = 8$
$2x - 8 = 3y$
$68/11 - 8 = 3y$
$68/11 - 88/11 = 3y$
$-20/11 = 3y$




2.

$5x+9y = 10$
$5x +3(2x-8) = 10$
$5x + 6x - 24 = 10$
$11x = 34$
$x = 34/11$

---

d.


1.
$4x+8 = 1 - 5y$
$4x + 5y = -7$ (2x = -4,5, y = 1)
$2(1-3y)+5y = -7$
$2 - 6y + 5 y = -7$
$2 - y = -7$
$-y = -9$
$y = 9$

2.
$3y + 2 = 3 - 2x$
$3y + 2x = 1$
$2x = 1 -3y$
$2x = 1 - 3*9$
$2x = 1 - 27$
$2x = -26$
$x = - 13$



zk
$3*9 + 2 = 3 - 2 * -13$
$27+2 = 3 + 26$
$true$

---

e.

1.

$xy-x = 2$
$y - x$

2.
$xy^2 -x = 6$

---
a. ????



$3x - \frac{4}{y-2} = 13$
$5x+3(y+2) = 20$

$15x - \frac{20}{y-2}=65$
$-15x - 9(y+2)=-60$



---
b.

1.
$\frac{x-1}{8}-\frac{y-7}{4}=1$
$x-1 -2y-14 = 8$
$x-2y = 23$
$x = 23 + 2y$
$x = 23 + -80/7$
$7x = 161 - 80$
$7x = 81$
$x = 81/7$



2.
$2x+\frac{2y-5}{3}=21$
$6x + 2y-5 = 63$
$6x + 2y = 58$
$3x + y = 29$
$3(23+2y)+y = 29$
$69 + 6y +y = 29$
$7y = 29 - 69$
$7y = -40$
$y = -\frac{40}{7}$

$81/7= 23 -80/7$
$81 = 161 - 80$
$161 = 161$ XD

---

c.

1.
$\frac{1}{x-2} + \frac{1}{y+3}=18$
$\frac{1}{-3-2}+\frac{1}{y+3}=18$
$1+\frac{-5}{y+3}=-90$
$y+3 + -5 = -90y - 270$
$y - 2 = -90y - 270$
$91y = -268$
$y = -268/91$


2.
$\frac{1}{x-2}-\frac{1}{x+3}=6$
$1 - \frac{x-2}{x+3} = 6x-12$
$x+3 - x-2 = (6x-12)(x+3)$
$1 = 6x^2+18x-12x-36$
$-6x^2 = 6x - 36$
$6x^2 + 6x = 36$
$x^2 + x = 6$
$-3 = x$


???????

---
d/

1.
$\frac{3}{x+1}+\frac{1}{y+3}=-1$
$3y+9 + x+1 = -1*(x+1)(y+3)$
$x +3y + 10 = -1 *(xy+3x+y+3)$
$x+3y+10 = -xy-3x-y-3$
$4x+4y+xy = -13$
$4x = -13 - 4y - xy$
$-13 - 4y - xy +4y+xy = -13$
$-13 = -13$
?????




2.
$\frac{1}{x+1}+\frac{1}{y-2}=-\frac{2}{3}$



---

$y_1 = 13/9$
$y_2 = -2$

$5x + 3(y+2) = 20$
$x_1 = 20 - 3y + 6$
$x_1 = 20 - 39/9 + 6$
$x_1 = 26/1 - 39/9$
$x_1 =$


---

$\frac{1}{x-2} = 18 - \frac{1}{y+3}$
$18-\frac{1}{y+3} - \frac{1}{x+3} = 6$
$-\frac{1}{y+3} - \frac{1}{x+3} = 6-18$
$-6 - \frac{1}{y+3} = -18 + \frac{1}{x+3}$
$6 + \frac{1}{y+3} = 18 - \frac{1}{x+3}$
---

$\frac{1}{x-2}+\frac{1}{y-3}=18$
$\frac{1}{x-2} - \frac{1}{y+3}=6$

$18y + 45 -1 = 6y + 18 + 1$
$18y + 44 = 6y + 19$
$12y +44 = 19$
$12y = 19 - 44$
$12y = -34$
$y = -17/6$