$(\log x-2)(\log x+4) = 0$
a = log x

$(a-2)(a+4)=0$

$a_1 = 2$
$a_2 = -4$


$x>0$
$x_1=100$ 
$x_2 = 0,001$


---


$log_4 x + \frac{1}{log_4x}-2=0$
D: $x > 0$
$log_4 x > 0$
$x \ne 1$

$log_4^2 x + 1 - 2log_4x = 0$
$t= log_4x$

$t^2 -2t + 1 = 0$
$(t-1)(t-1) = 0$
$log_4 x = 1$
$x =4^1$
$x = 4$

---


$(log_5 u)^{-1} -2 = -log_5 u$
$\frac{1}{log_5u}-2 = -log_5 u$
D: 
$log_5u > 0$
$u >0$
$u \ne 1$



$\frac{1}{t}-2=-t$
$1-2t=-t^2$
$t^2-2t+1=0$
$t=1$
$log_5u=1$
$u=5^1$
$5=u$

---


$ln x -1 = \frac{12}{lu x}$
$ln x = r$
$r-1=12/r$
$r^2-r=12$
$r^2-r-12=0$$
$(r+3)(r-4) = 0$
$r_1 = -3$
$r_2 = 4$

$x_1= e^{-3}$
$x_2=e^4$

$D:$
$x >0$
$lnx>0$
$x \ne 1$


---

$1+log_8(x)=log_8(6-x)+2log_8(x)$
$1=log_8(6-x)+2log_8(x) - log_8(x)$
$1+log_8(x) = log_8(6-x)+log_8(x^2)$
$8x=6x^2-x^3$
$x^3-6x^2+8x = 0$  /x
$x(x^2-6x+8) = 0$
$x = 0$
$x^2-6x+8 = 0$
$x_1 = 2, x_2 = 4$
p:
$x > 0$
$6-x > 0$
$-x > -6$
$x < 6$

$\mathbb{K} = {2,4}$


---

$log(x)-2 = 6log^{-1}(x)-1$
$log(x)= P$
$P-2=\frac{6}{P}-1$
$P^2-P-6=0$
$()()$